store/client_proofs/store.v
@@ -37,7 +37,8 @@ Lemma wp_client_send_store c kI kR cs t1 t2 t2' :
   {{{ RET #(); client_connected kI kR cs ∗ rem_mapsto kI kR t1 t2' }}}.
 Proof.
 iIntros "#chan_c (_ & _ & #? & _) #p_t1 #p_t2' !> %Φ [client mapsto] post".
-iDestruct "client" as "(%n & %beginning & <- & <- & #conn & ts & client)".
+iDestruct "client"
+  as "(%n & %beginning & <- & <- & %e_rl & #conn & ts & client)".
 iMod (rem_mapsto_update t2' with "client mapsto")
   as "(client & mapsto & #update)".
 wp_lam. wp_pures.
@@ -47,7 +48,8 @@ iPoseProof (store_predI with "client update") as "#?".
 wp_pures. wp_list. wp_bind (tint _). iApply wp_tint. wp_list.
 wp_term_of_list. wp_pures.
 iApply (wp_connection_send with "[//] [//] [] [#] conn") => //.
-- rewrite public_of_list /= public_TInt. by eauto.
+{ rewrite public_of_list /= public_TInt. by eauto. }
+{ by iIntros "!> _". }
 iIntros "!> _".
 iApply ("post" with "[ts client mapsto]").
 by iFrame; eauto.
@@ -61,7 +63,8 @@ Lemma wp_client_ack_store c kI kR cs :
   {{{ RET #(); client_connected kI kR cs }}}.
 Proof.
 iIntros "#chan_c (_ & _ & _ & #? & _) !> %Φ client post".
-iDestruct "client" as "(%n & %beginning & <- & <- & #conn & ts & client)".
+iDestruct "client"
+  as "(%n & %beginning & <- & <- & %e_rl & #conn & ts & client)".
 rewrite /Client.ack_store. wp_pures.
 wp_apply (wp_connection_timestamp with "ts"). iIntros "ts".
 wp_pures.
