store/server_proofs/load.v
@@ -31,6 +31,7 @@ Variable N : namespace.
 Ltac failure := iLeft; iFrame.
 
 Lemma wp_server_handle_load c cs ldb db n :
+  cs_role cs = Resp →
   channel c -∗
   store_ctx N -∗
   handler_correct
@@ -40,10 +41,10 @@ Lemma wp_server_handle_load c cs ldb db n :
     (N.@"load", Server.handle_load N c (repr cs) ldb)
     n.
 Proof.
-iIntros "#chan_c #ctx".
+iIntros "%e_rl #chan_c #ctx".
 iPoseProof (store_ctx_load with "ctx") as "?".
 iPoseProof (store_ctx_ack_load with "ctx") as "?".
-rewrite /handler_correct. wp_lam; wp_pures.
+rewrite /handler_correct e_rl /=. wp_lam; wp_pures.
 iModIntro. iExists _. iSplit => //. iIntros "!> %m _ #p_m #conn ts (server & db)".
 wp_pures.
 wp_bind (Connection.timestamp _).
@@ -62,6 +63,7 @@ wp_pures.
 iPoseProof (ack_load_predI db_t1 with "server") as "#[??]".
 wp_bind (Connection.send _ _ _ _).
 iApply (wp_connection_send with "[//] [//] [] [] conn") => //.
+{ by iIntros "!> _". }
 iIntros "!> _". wp_pures. iModIntro.
 iRight. iExists _. iSplit => //. iExists _, _. iLeft. by iFrame.
 Qed.
